\documentclass{article}
\usepackage{amsmath}
\usepackage{tocloft} % For customizing the table of contents

\title{Criteria and proof for when a new view must be appended in a Tinygrad shapeTracker}
\author{Peter Schillinger}
\date{September 2024}

% Disable paragraph indentation for the entire document
\setlength{\parindent}{0pt}

\begin{document}

\maketitle
\tableofcontents % Generates the table of contents

\section{Definitions}

\begin{flushleft}
\textbf{Definition:} A \textbf{view} is defined as a pair \((\vec{k}, \vec{s})\), where:
\end{flushleft}
\[
\vec{k} = (k_1, k_2, \ldots, k_n), and \quad \vec{s} = (s_1, s_2, \ldots, s_n)
\]


\textbf{Definition:} The \textbf{view order} is an ordering of the tensor's elements associated with that view. For the first view in a shapeTracker, the view order is the order of elements stored statically in memory. For our purposes we will identify elements by their index (starting from 0) in the view order. 

\begin{flushleft}
\textbf{Definition:} Given a shape $\vec{k} = (k_1, k_2, \ldots, k_n)$, define the \textbf{mixed radix conversion function} to be the function: $R_{\vec{k}} : \mathbb{N} \rightarrow \mathbb{N}^n$, with domain $\{0, 1, \ldots, (\prod_{l=1}^n k_l) - 1\}$.
\end{flushleft}

\[
R_{\vec{k}}(i) = 
\begin{pmatrix}
\left\lfloor \frac{i}{\prod_{l=2}^{n} k_l} \right\rfloor \bmod k_1 \\
\vdots \\
\left\lfloor \frac{i}{k_n} \right\rfloor \bmod k_{n-1} \\
i \bmod k_n
\end{pmatrix}
= 
\begin{pmatrix}
\left\lfloor \frac{i}{\prod_{l=j+1}^{n} k_l} \right\rfloor \bmod k_j
\end{pmatrix}_{j=1}^n
\]

\begin{flushleft}
\textbf{Definition:} Given a view $(\vec{k}, \vec{s})$, the \textbf{reshape order} is the permutation of size n, defined as the composition of $R_{\vec{k}}$ and the matrix multiplication of $A = [s_1 \, s_2 \, \ldots \, s_n]$. That is, the ith element in the reshape order is given by 

\[
A(R_{\vec{k}}(i))
\]
for i in $\{0, 1, \ldots, (\prod_{l=1}^n k_l) - 1\}$. If the tensor has not been permuted, the reshape order is the identity permutation.
\end{flushleft}

\textbf{Definition:} Given a view $\vec{k} = (k_1, k_2, \ldots, k_n)$, $\vec{s} = (s_1, \ldots, s_n)$, define the \textbf{max merge partition} to be the partition 
\[
\vec{p} = (p_1 = 1, p_2, \ldots, p_{q})
\]
to be such that for all integers $j \in \{ 1, \ldots, n \}$ where $p_i < j < p_{i+1}$ for some $i \in \{ 1, \ldots, q - 1 \}$,

\[
s_j \cdot k_j = s_{j-1}
\]
and for all $i \in \{ 1, \ldots, q \}$
\[
\quad s_{p_i} \cdot k_{p_i} \neq s_{p_i - 1} \quad
\]

\textbf{Definition:} Given such a view and max merge partition, define the \textbf{max merge view} to have shape 
\[
\vec{m} = (m_1, \ldots, m_{q})
\]
and strides 
\[
\vec{t} = (t_1, \ldots, t_{q}),
\]
where, for $i \in \{ 1, \ldots, q \}$,
\[
m_i = \prod_{\ell = p_i}^{p_{i+1}-1} k_{\ell} \quad \text{(where $p_{q + 1} = n + 1$)}
\]
and
\[
t_i = s_{p_{i+1} - 1} \quad \text{(where again $p_{q + 1} = n + 1$)}.
\]




\section{Proof of Mergeability Altering Within Contiguous Subblocks}

\subsection{Splitting Any Dimension}

Given a view $\vec{k}_1 = (k_1, k_2, \ldots, k_n)$ and $\vec{s}_1 = (s_1, s_2, \ldots, s_n)$, we show that for any $j \in \{1, \ldots, n\}$ and any factors $p_1$ and $p_2$ of $k_j$, i.e., $p_1 \cdot p_2 = k_j$, reshaping to a new shape 
\[
\vec{k}_2 = (k_1, k_2, \ldots, k_{j-1}, p_1, p_2, k_{j+1}, \ldots, k_n) := (c_1, \ldots, c_{n+1})
\]
need not append a new view.

\textbf{Proof:}
To show that a new view need not be appended, we must show that there exists a linear function from the indices of the new shape to the reshape order. Let $A_1 : \mathbb{N}^n \rightarrow \mathbb{N}$ be the linear function mapping the old indices to the reshape order, i.e., $A_1 = [s_1 \, \ldots \, s_n]$. Then we are to show that there exists some $A_1$ such that, for all i in $\{0, 1, \ldots, (\prod_{l=1}^n k_l) - 1\}$,

\[A_1(R_{\vec{k_1}}(i)) = A_2(R_{\vec{k_2}}(i))
\].
Computing the left hand side,
\[A_1(R_{\vec{k_1}}(i))=A_1(\begin{pmatrix}
\left\lfloor \frac{i}{\prod_{l=2}^{n} k_l} \right\rfloor \bmod k_1 \\
\vdots \\
\left\lfloor \frac{i}{k_n} \right\rfloor \bmod k_{n-1} \\
i \bmod k_n
\end{pmatrix})=\sum_{r=1}^{n} s_r \left( \left\lfloor \frac{i}{\prod_{l=r+1}^{n} k_l} \right\rfloor \bmod k_r \right)
\]

We claim that $A_2 = \vec{s}_2^{\top} = [s_1, s_2, \ldots, s_{j-1}, p_2 \cdot s_j, s_j, s_{j+1}, \ldots, s_n] := [t_1, \ldots, t_{n+1}]$ works.

Computing the right hand side gives
\[A_2(R_{\vec{k_2}}(i))=A_2(\begin{pmatrix}
\left\lfloor \frac{i}{\prod_{l=2}^{n+1} c_l} \right\rfloor \bmod c_1 \\
\vdots \\
\left\lfloor \frac{i}{c_{n+1}} \right\rfloor \bmod c_{n} \\
i \bmod c_{n+1}
\end{pmatrix})=\sum_{r=1}^{n+1} t_r \left( \left\lfloor \frac{i}{\prod_{l=r+1}^{n+1} k_l} \right\rfloor \bmod c_r \right)
\]
Cancelling like terms on each side, we find we are only left with
\[
s_{j} \left( \left\lfloor \frac{i}{\prod_{l=j+1}^{n} k_{l}} \right\rfloor \bmod k_{j} \right) = t_{j} \left( \left\lfloor \frac{i}{\prod_{l=j+1}^{n+1} c_{l}} \right\rfloor \bmod p_{1} \right) + t_{j+1} \left( \left\lfloor \frac{i}{\prod_{l=j+2}^{n+1} c_{l}} \right\rfloor \bmod p_{2} \right)
\]

\vspace{0.5em}

\[
\phantom{s_{j} \left( \left\lfloor \frac{i}{\prod_{l=j+1}^{n} k_{l}} \right\rfloor \bmod k_{j} \right) =} 
=p_2 \cdot s_j \left( \left\lfloor \frac{i}{\prod_{l=j+1}^{n+1} c_{l}} \right\rfloor \bmod p_{1} \right) + s_j \left( \left\lfloor \frac{i}{\prod_{l=j+1}^{n} k_{l}} \right\rfloor \bmod p_{2} \right)
\]
Dividing out by $s_j$ and setting $w=\frac{i}{\prod_{l=j+1}^{n} k_{l}}$ we get 
\[
\lfloor{w}\rfloor \bmod k_j = p_2 \left( \left\lfloor \frac{w}{p_2} \right\rfloor \bmod p_1 \right) + \left(\lfloor{w}\rfloor \bmod p_2 \right) \tag{1}
\]

Let $r_2 = \lfloor w \rfloor \bmod p_2$. Then
\[
\lfloor w \rfloor = p_2 \left\lfloor \frac{w}{p_2} \right\rfloor + r_2
\]

Let $\left\lfloor \frac{w}{p_2} \right\rfloor = r_1 \bmod p_1$. Then
\[
\left\lfloor \frac{w}{p_2} \right\rfloor = p_1 m + r_1 \quad \text{for some integer } m.
\]

Therefore,
\[
\lfloor w \rfloor = p_2 \lfloor \frac{w}{p_2} \rfloor + r_2
\]
\[
= p_2 \left( p_1 m + r_1 \right) + r_2
\]
\[
= p_1 p_2 m + p_2 r_1 + r_2
\]
\[
= k_j m + p_2 r_1 + r_2
\]
\[
= p_2 r_1 + r_2 \bmod k_j
\]

But
\[
p_2 \left( \left\lfloor \frac{w}{p_2} \right\rfloor \bmod p_1 \right) + \left( \lfloor w \rfloor \bmod p_2 \right) = p_2 r_1 + r_2 \quad \text{by definition.}
\]
\[
\Rightarrow \quad \text{LHS} = \text{RHS}
\]

\[
\text{Done } \# 
\]



\subsection{Combining Dimension Within Contiguous Subblock}

Given view 
\[
\vec{k}_1 = (k_1, k_2, \ldots, k_n), \quad  \quad \vec{s}_1 = (s_1, s_2, \ldots, s_n),
\]
we show that for any $j \in \{2, \ldots, n\}$, if $s_j k_j = s_{j-1}$, then reshaping to 
\[
\vec{k}_2 = (k_1, \ldots, k_{j-2}, k_{j-1} \cdot k_{j}, k_{j+1}, \ldots, k_n) := (c_1, \ldots, c_{n-1}),
\]
need not append a new view, i.e., there exists a linear function from indices in $\vec{k}_2$ to reshape order.

\textbf{Proof:}

Let $A_1$ be a linear function for shape $\vec{k}_1$. We show there exists a linear function $A_2$ such that
\[
A_1 \left( R_{\vec{k}_1}(i) \right) = A_2 \left( R_{\vec{k}_2}(i) \right) \quad \text{for all } i \in \left\{ 0, \ldots, \prod_{i=1}^n k_i - 1 \right\}.
\]

Let $A_2 = \vec{s}_2^{T} = \begin{bmatrix}
s_1, \ldots, s_{j-2}, s_j, s_{j+1}, \ldots, s_n
\end{bmatrix}:= \begin{bmatrix}
t_1, \ldots, t_{n-1}
\end{bmatrix}.

We want to show
\[
A_1 \left( R_{\vec{k}_1}(i) \right) = A_2 \left( R_{\vec{k}_2}(i) \right) \quad \text{for all } i \in \left\{ 0, \ldots, \prod_{i=1}^n k_i - 1 \right\}
\]

Simplifying both sides gives
\[
\sum_{r=1}^{n} s_r \left( \left\lfloor \frac{i}{\prod_{l=r+1}^{n} k_l} \right\rfloor \mod k_r \right) = \sum_{r=1}^{n-1} t_r \left( \left\lfloor \frac{i}{\prod_{l=r+1}^{n-1} c_l} \right\rfloor \mod c_r \right)
\]

And cancelling like terms gives
\[
s_{j-1} \left( \left\lfloor \frac{i}{\prod_{l=j}^{n} k_l} \right\rfloor \mod k_{j-1} \right) + s_j \left( \left\lfloor \frac{i}{\prod_{l=j+1}^{n} k_l} \right\rfloor \mod k_j \right) = t_{j-1} \left( \left\lfloor \frac{i}{\prod_{l=j}^{n-1} c_l} \right\rfloor \mod k_{j-1}k_{j} \right)
\]

But because $t_{j-1} = s_{j}$, $s_{j-1}=s_{j}k_{j}$, and letting $w = \left \frac{i}{\prod_{l=j+1}^{n} k_l} \right$, we recover an equivalent equation to (1):
\[
k_j \left( \left\lfloor \frac{w}{k_j} \right\rfloor \mod k_{j-1} \right) + \left( \lfloor w \rfloor \mod k_j \right) = \lfloor w \rfloor \mod k_{j-1}k_j
\]

which was shown to hold.

\[
\text{Done } \#
\]

\subsection{Proof of Mergeability of Arbitrary Altering Inside of Contiguous Subblocks}

Given a view $\vec{k} = (k_1, \ldots, k_n)$, $\vec{s} = (s_1, \ldots, s_n)$ and a new shape $\vec{u} = (u_1, \ldots, u_n)$ for which there exists a partition $\vec{p} = (p_1 = 1, p_2, \ldots, p_q)$ such that for all $i \in \{1, \ldots, q\}$,
\[
\prod_{l=p_i}^{p_{i+1}-1} \mu_l = m_i,
\]
where $m_i$ is the $i$th size in the max merge viewâ€™s shape $\vec{m} = (m_1, \ldots, m_q)$ associated with $(\vec{k}, \vec{s})$.

\textbf{Proof:}

By iteratively combining all dimensions to the view's max merge shape (shown in 2.2), and then splitting $m_i$ into arbitrary factors $\mu_{p_i}, \mu_{p_i+1}, \ldots, \mu_{p_{i+1}-1}$ (shown in 2.1), we can reshape to $\vec{u}$ without ever appending a view.

\[
\text{Done } \#
\]


\section{Disproof of Mergeability Altering Outside of Contiguous Subblocks}

Given view $(\vec{u}, \vec{v})$ and associated max merge view $(\vec{m}, \vec{s})$, let $\vec{k} = (k_1, \ldots, k_n)$ be such that $\prod k_\ell = \prod u_\ell$, but there exists no partition $\vec{p} = (p_1, \ldots, p_\ell)$ such that
\[
m_i = \prod_{l = p_i}^{p_{i+1}-1} k_l \quad \forall i \in \{1, \ldots, q\}.
\]

We show that reshaping to $\vec{k}$ necessarily appends view, that is, that the function from indices in $\vec{k}$ to reshape order is nonlinear.

\textbf{Proof:}

Imagine accumulating the $k$'s in $\vec{k}$, starting at $k_n$ and going backwards and keeping track of the cumulative product.

If there is no partition, then there must exist some first index $j$ such that
\[
\prod_{\ell=j+1}^{n} k_\ell < \prod_{\ell=i}^{q} m_\ell < \prod_{\ell=j}^{n} k_\ell \quad \text{where } i \text{ is chosen to be maximal.}
\]

But because $j$ is the first index where this happens and $i$ is maximal,
\[
\prod_{\ell=i+1}^{q} m_\ell = \prod_{\ell=p}^{n} k_\ell \quad \text{for some } p \in \{j+1, \ldots, n\}.
\]

And of course, because $i$ is maximal
\[
\prod_{\ell=i+1}^{q} m_\ell \leq \prod_{\ell=j+1}^{n} k_\ell.
\]

Let $A_0 = \vec{v}^{\top}$ be the given linear function for the shape $\vec{u}$. 

Towards a contradiction, assume there exists some linear function $A_2$ such that 
\[
A_0 \left( R_{\vec{u}}(i) \right) = A_2 \left( R_{\vec{k}}(i) \right) \quad \forall i \in \left\{0, \ldots, \prod_{\ell=1}^{n} k_\ell - 1\right\}.
\]

Because we have shown mergeability to max merged shape, we know, for $A_1 = \vec{s}^T = [s_1, \ldots, s_\ell]$,
\[
A_0 \left( R_{\vec{u}}(i) \right) = A_1 \left( R_{\vec{m}}(i) \right) \quad \text{where } \vec{u}
\]

\[
\Rightarrow A_1 \left( R_{\vec{m}}(i) \right) = A_2 \left( R_{\vec{k}}(i) \right)
\]

Let $A_2 = (t_1, \ldots, t_n)$.

For $a \in \{j+1, j+2, \ldots, p\}$, let the number
\[
n_a = \prod_{l=a}^{n} k_l = (\prod_{l=i+1}^{q} m_l) (\prod_{l=a}^{p-1} k_l) < \prod_{l=i}^{q} m_l \quad \text{(where } \prod_{l=p}^{p-1} k_l = 1 \text{ of course).}
\]

Then
\[
R_{\vec{m}}} (n_a) = 
\begin{pmatrix}
0 \\
0 \\
\vdots \\
\left( \left\lfloor \frac{(\prod_{l=i+1}^{q} m_l) (\prod_{l=a}^{p-1} k_l)}{\prod_{l=i+1}^{q} m_l} \right\rfloor \bmod m_i \right) \quad  \\
\vdots \\
0
\end{pmatrix}
= 
\begin{pmatrix}
0 \\
0 \\
\vdots \\
 \left\prod_{l=a}^{p-1} k_l  \\
\vdots \\
0
\end{pmatrix}
\]

and

\[
R_{\vec{k}} (n_a) = 
\begin{pmatrix}
0 \\
0 \\
\vdots \\
1\\
\vdots \\
0
\end{pmatrix}
\text{where the 1 appears in the (a-1)th entry} 
\]

Of course
\[
A_1 \left( R_{\vec{m}}(n_a) \right) = A_2 \left( R_{\vec{k}}(n_a) \right)
\]
still holds.

But 
\[
A_1 \left( R_{\vec{m}}(n_a) \right) = s_i \prod_{l=a}^{p-1} k_l \quad \text{and} \quad A_2 \left( R_{\vec{k}}(n_a) \right) = t_{a-1}.
\]

\[
\Rightarrow \quad t_{a-1} = s_i \prod_{l=a}^{p-1} k_l.
\]

Now consider the number
\[
n_0 = \prod_{l=i}^{q} m_l = m_i \prod_{l=p}^{n} k_l.
\]

\[
R_{\vec{m}}(n_0) = 
\begin{pmatrix}
0 \\
0 \\
\vdots \\
0 \\
1 \quad \text{($i$-th spot)} \\
0 \\
\vdots \\
0
\end{pmatrix}
\]

and

\[
R_{\vec{k}}(n_0) = 
\begin{pmatrix}
0 \\
\vdots \\
0 \\
 \left\lfloor \frac{m_i}{\prod_{l=j+1}^{p-1} k_l} \right\rfloor \bmod k_j \\
 \vdots \\
 \left\lfloor \frac{m_i}{k_{p-1}} \right\rfloor \bmod k_{p-2} \\
m_i \bmod k_{p-1} \\
0 \\
\vdots \\
0 \\
\end{pmatrix}
\]

We again have $A_1 \left( R_{\vec{m}}(n_0) \right) = A_2 \left( R_{\vec{k}}(n_0) \right)$.

But
\[
A_1 \left( R_{\vec{m}}(n_0) \right) = s_{i-1}
\]
and
\[
A_2 \left( R_{\vec{k}}(n_0) \right) = \sum_{r=p-1}^{j} t_r \left( \left\lfloor \frac{m_i}{\prod_{l=r+1}^{p-1} k_l} \right\rfloor \bmod k_r \right) 
\]
\[
= s_i\sum_{r=p-1}^{j} \prod_{l=r+1}^{p-1} k_l \left(  \left\lfloor \frac{m_i}{\prod_{l=r+1}^{p-1} k_l} \right\rfloor \mod k_r \right)
\]
\[
= s_i\cdot m_i.
\]

\[
\Rightarrow \quad s_{i-1} = s_i m_i \text{, which violates the definition of a max merged shape}\quad
\]
\[
\Rightarrow \quad A_2 \text{ is not linear, and therefore reshaping to } \vec{k} \text{ without appending a view is impossible.} \quad  
\]
\[
\text{Done} \, \#
\]

\end{document}
